Work on simulation

Simu.v
@@ -119,10 +119,10 @@ Inductive exp_eval (me: menv) (ve: venv): exp -> val -> Prop :=
     forall x v ty,
       PM.MapsTo x v ve ->
       exp_eval me ve (Var x ty) v
-(* | estate: *)
-(*     forall x v ty, *)
-(*       mfind_mem x me = Some v -> *)
-(*       exp_eval me ve (State x ty) v *)
+| estate:
+    forall x v ty,
+      mfind_mem x me = Some v ->
+      exp_eval me ve (State x ty) v
 | econst:
     forall c ty,
       exp_eval me ve (Const c ty) (val_of_const c).
@@ -136,15 +136,12 @@ Inductive stmt_eval :
     exp_eval me ve e v ->
     PM.add x v ve = ve' ->
     stmt_eval prog (me, ve, Assign x e) (me, ve', Skip)
-(* | Iassignst: *)
-(*   forall prog me ve x e v me', *)
-(*     exp_eval me ve e v -> *)
-(*     madd_mem x v me = me' -> *)
-(*     stmt_eval prog (me, ve, AssignSt x e) (me', ve, Skip) *)
-(* | Iskip: *)
-(*     forall prog menv env, *)
-(*       stmt_eval prog (menv, env) Skip (menv, env). *)
-.
+| Iassignst:
+  forall prog me ve x e v me',
+    exp_eval me ve e v ->
+    madd_mem x v me = me' ->
+    stmt_eval prog (me, ve, AssignSt x e) (me', ve, Skip).
+
 (** ** Determinism of semantics *)
 
 Theorem exp_eval_det:
@@ -154,8 +151,8 @@ Theorem exp_eval_det:
     v1 = v2.
 Proof.
   induction e; intros v1 v2 H1 H2;
-  inversion H1 as [xa va tya Hv1(* |xa va tya Hv1 *)|ca tya Hv1];
-  inversion H2 as [xb vb tyb Hv2(* |xb vb tyb Hv2 *)|cb tyb Hv2];
+  inversion H1 as [xa va tya Hv1|xa va tya Hv1|ca tya Hv1];
+  inversion H2 as [xb vb tyb Hv2|xb vb tyb Hv2|cb tyb Hv2];
   try (unfold PM.MapsTo in *; rewrite Hv1 in Hv2; (injection Hv2; trivial) || apply Hv2); subst.
   reflexivity.
 Qed.
@@ -283,6 +280,9 @@ Section PRESERVATION.
   Let tge := Clight.globalenv tprog.
 
   (* Hypothesis VE_IN_VARS: forall x v (ve: venv), PM.MapsTo x v ve -> exists t, In (x, t) prog.(p_vars). *)
+
+  Definition chunk_of_typ ty := AST.chunk_of_type (Ctypes.typ_of_type ty).
+  Definition pointer_of_node node := pointer_of (type_of_inst node).
   
   Definition main_fun :=
     Clight.mkfunction Ctypes.type_int32s AST.cc_default []
@@ -297,13 +297,13 @@ Section PRESERVATION.
     destruct c; simpl; reflexivity.
   Qed.
 
-  Lemma type_of_val:
-    forall me ve e v,
-      exp_eval me ve e v ->
-      Values.Val.has_type v (Ctypes.typ_of_type (typeof e)).
-  Proof.
-    induction 1; simpl; admit.
-  Qed.
+  (* Lemma type_of_val: *)
+  (*   forall me ve e v, *)
+  (*     exp_eval me ve e v -> *)
+  (*     Values.Val.has_type v (Ctypes.typ_of_type (typeof e)). *)
+  (* Proof. *)
+  (*   induction 1; simpl; admit. *)
+  (* Qed. *)
   
   Lemma sem_cast_same:
     forall v t t',
@@ -325,7 +325,7 @@ Section PRESERVATION.
       try contradiction; try now contradict U.
   Qed.
 
-  Lemma build_co_ok:
+  (*Lemma build_co_ok:
     Ctypes.build_composite_env (map translate_class prog.(p_cls)) = Errors.OK (Clight.genv_cenv tge).
   Proof.
     unfold translate in TRANSL.
@@ -335,7 +335,7 @@ Section PRESERVATION.
 
   Hypothesis BUILD_CO_OK:
     Ctypes.build_composite_env (map translate_class prog.(p_cls)) = Errors.OK (Clight.genv_cenv tge).
-
+  
   Remark find_class_name:
     forall id cls c cls',
       find_class id cls = Some (c, cls') ->
@@ -356,39 +356,24 @@ Section PRESERVATION.
               exists delta,
                 Ctypes.field_offset (Clight.genv_cenv tge) x (Ctypes.co_members co) = Errors.OK delta).
   Proof.
-    assert (tprog.(Clight.prog_types) = map translate_class prog.(p_cls)) as H.
-    - admit.
-    - destruct MAINNODE as [c [cls Hcls]].
-      assert (In (translate_class c) tprog.(Clight.prog_types)) as Hin.
-      + clear MAINNODE BUILD_CO_OK.
-        induction (Clight.prog_types tprog); induction (p_cls prog); simpl in *. 
-        * discriminate.
-        * apply nil_cons in H; contradiction.
-        * symmetry in H; apply nil_cons in H; contradiction.            
-        *{ destruct (ident_eqb (c_name a0) main_node).
-           - inversion Hcls; subst.
-             inversion H. now left.
-           - inversion H; subst.
-             right. apply IHl. admit. (* how to do the induction ??? *)
-         }
-        (* induction prog.(p_cls). *)
-        (* * simpl in *; discriminate. *)
-        (* *{ simpl in *. *)
-        (*    destruct (ident_eqb (c_name a) main_node). *)
-        (*    - inversion_clear Hcls; subst. *)
-        (*      apply in_eq. *)
-        (*    - specialize (IHl Hcls tprog). *)
-        (*      apply in_cons. *)
-        (*  } *)
-      + rewrite H in Hin.
-        unfold translate_class at 1 in Hin.
-        apply find_class_name in Hcls.
-        destruct c; simpl in Hcls; subst.
-        pose proof (Ctypes.build_composite_env_charact _ _ _ _ _ _ BUILD_CO_OK Hin) as [co Hco].
-        exists co; split.
-        * tauto.
-        * intros ** Hx.
-          admit.                (* how to get a witness ??? *)
+    destruct MAINNODE as [c [cls Hcls]].
+    assert (In (translate_class c) (map translate_class prog.(p_cls))) as Hin.
+    - clear TRANSL MAINNODE BUILD_CO_OK.
+      apply in_map.
+      induction (p_cls prog); simpl in *.
+      + discriminate.
+      + destruct (ident_eqb (c_name a) main_node).
+        * inversion Hcls; subst.
+          now left.
+        * right. now apply IHl.
+    - unfold translate_class in Hin.
+      apply find_class_name in Hcls.
+      destruct c; simpl in Hcls; subst.
+      pose proof (Ctypes.build_composite_env_charact _ _ _ _ _ _ BUILD_CO_OK Hin) as [co Hco].
+      exists co; split.
+      * tauto.
+      * intros ** Hx.
+        admit.                (* how to get a witness ??? *)
   Qed.
 
   Inductive tr_vars: Clight.env -> Prop :=
@@ -408,47 +393,70 @@ Section PRESERVATION.
   (*     legit_type (Ctypes.Tlong sign attr)  *)
   (* | legit_tfloat: forall size attr, *)
   (*     legit_type (Ctypes.Tfloat size attr). *)
-  
+   *)
+
+  Axiom wt_state_pred: ident * typ -> program -> Prop.
   Inductive well_typed_exp: exp -> Prop :=
   | wt_var: forall x ty,
-      (* legit_type ty -> *)
       In (x, ty) prog.(p_vars) ->
       well_typed_exp (Var x ty)
+  | wt_state: forall x ty,
+      wt_state_pred (x, ty) prog ->
+      well_typed_exp (State x ty)
   | wt_const: forall c ty,
-      (* legit_type ty -> *)
       well_typed_exp (Const c ty).
 
   Inductive well_typed: stmt -> Prop :=
   | wt_assign: forall x e,
+      In (x, typeof e) prog.(p_vars) ->
       well_typed_exp e ->
       well_typed (Assign x e)
+  | wt_stassign: forall x e,
+      wt_state_pred (x, typeof e) prog ->
+      well_typed_exp e ->
+      well_typed (AssignSt x e)
   | wt_skip: well_typed Skip.
-  
-  Inductive well_assigned_exp: exp -> Prop :=
-  | wa_var: forall x ty,
-      (exists m, forall chunk loc v m', Memory.Mem.store chunk m loc 0 v = Some m') ->
-      well_assigned_exp (Var x ty)
-  | wa_const: forall c ty,
-      well_assigned_exp (Const c ty).
-  
-  Inductive well_assigned: stmt -> Clight.env -> Prop :=
-  | wa_assign: forall x e env loc,
-      well_assigned_exp e ->
-      Maps.PTree.get x env = Some (loc, typeof e) ->
-      well_assigned (Assign x e) env
-  | wa_skip: forall env,
-      well_assigned Skip env.
 
-  Inductive compat_mem: menv -> venv -> Memory.Mem.mem -> Prop :=
-    compat_mem_intro: forall menv venv mem,
-      compat_mem menv venv mem.
+  (*
+  Inductive well_assigned_exp: Memory.Mem.mem -> (* AST.memory_chunk -> *) exp -> (* val -> *) Prop :=
+  wa_intro: forall m' e,
+      (forall m chunk loc ofs v, Memory.Mem.store chunk m' loc ofs v = Some m) ->
+      well_assigned_exp m' e.
+  
+  Inductive well_assigned: Clight.env -> Memory.Mem.mem -> stmt -> Prop :=
+  | wa_assign: forall x e m env loc,
+      well_assigned_exp m e ->
+      Maps.PTree.get x env = Some (loc, typeof e) ->
+      well_assigned env m (Assign x e)
+  | wa_skip: forall env m,
+      well_assigned env m Skip.
+
+  Inductive well_evaluated_exp: menv -> venv -> exp -> Prop :=
+  | we_intro: forall e me ve v,
+      Ctypes.access_mode (typeof e) = Ctypes.By_value (chunk_of_typ (typeof e)) ->
+      v <> Values.Vundef ->
+      Values.Val.has_type v (Ctypes.typ_of_type (typeof e)) ->
+      Values.Val.load_result (chunk_of_typ (typeof e)) v = v ->
+      exp_eval me ve e v ->
+      well_evaluated_exp me ve e.
+
+  Inductive well_evaluated: menv -> venv -> stmt -> Prop :=
+    | we_assign: forall x e me ve,
+        well_evaluated_exp me ve e ->
+        well_evaluated me ve (Assign x e)
+    | we_skip: forall me ve,
+        well_evaluated me ve Skip.
+  
+  Definition compat_mem (me: menv) (ve: venv): Memory.Mem.mem :=
+    Memory.Mem.empty.
     
   Inductive match_states: state -> Clight.state -> Prop :=
     state_intro: forall menv venv s k env lenv mem,
       tr_vars env ->
       well_typed s ->
-      well_assigned s env ->
-      compat_mem menv venv mem ->
+      well_assigned env mem s ->
+      well_evaluated menv venv s ->
+      compat_mem menv venv = mem ->
       match_states
         (menv, venv, s)
         (Clight.State main_fun (translate_stmt main_node s) k env lenv mem).
@@ -505,30 +513,30 @@ Section PRESERVATION.
                         (at level 67).
 
   
-  Hint Constructors Clight.eval_lvalue well_typed well_assigned match_states.
+  Hint Constructors Clight.eval_lvalue Clight.eval_expr well_typed well_assigned well_evaluated match_states.
   
   Lemma expr_eval:
-    forall me ve exp v chunk e le m',
+    forall me ve exp v chunk e le m' m,
       tr_vars e ->
       well_typed_exp exp ->
-      well_assigned_exp exp ->
+      well_assigned_exp m' exp ->
       Values.Val.load_result chunk v = v ->
       Ctypes.access_mode (typeof exp) = Ctypes.By_value chunk ->
       exp_eval me ve exp v ->
-      Clight.eval_expr tge e le m' (translate_exp main_node exp) v.
+      Clight.eval_expr tge e le m (translate_exp main_node exp) v.
   Proof.
     intros me ve exp;
     induction exp as [x ty|x ty|c ty];
     intros ** Hvars Hwt Hwa Hload Haccess Heval;
     inversion Heval as [? ? ? Hmto(* |? ? ? Hmem *)|];
     inversion Hwt as [? ? Hin|];
-    inversion Hwa as [? ? [m Hstore]|];
+    inversion Hwa as [? ? Hstore];
     revert Hload; subst; simpl in *; intro Hload.    
-    - destruct (tr_env_in _ _ _ _ _ Hmto Hin Hvars) as [loc Hget].  
-      apply Clight.eval_Elvalue with (loc:=loc) (ofs:=Int.zero); eauto.
+    - destruct (tr_env_in _ _ _ _ _ Hmto Hin Hvars) as [loc Hget].
+      apply Clight.eval_Elvalue with (loc:=loc) (ofs:=Int.zero); auto.
       eapply Clight.deref_loc_value; eauto.
       rewrite <-Hload.
-      now apply Memory.Mem.load_store_same with m.         
+      eapply Memory.Mem.load_store_same; eauto.         
     (* - assert (loc: Values.block). admit. *)
     (*   assert (ofs: Int.int). admit. (* where are they comin' from ??? *) *)
     (*   destruct tr_main_node as [co [Hco Hdelta]]. *)
@@ -547,9 +555,127 @@ Section PRESERVATION.
     (*      } *)
     (*   + eapply Clight.deref_loc_value; eauto. simpl. admit. (* LOAD *) *)
     - destruct c; constructor.
+  Qed.*)
+
+  Definition valid_val (v: val) (t: typ): Prop :=
+     Ctypes.access_mode t = Ctypes.By_value (chunk_of_typ t)
+     /\ v <> Values.Vundef
+     /\ Values.Val.has_type v (Ctypes.typ_of_type t).
+
+  Definition compat_venv (ve: venv) (env: Clight.env) (m: Memory.Mem.mem):  Prop :=
+    forall x t v,
+      PM.MapsTo x v ve ->
+      exists loc,
+        Maps.PTree.get x env = Some (loc, t)
+        /\ Memory.Mem.load (chunk_of_typ t) m loc 0 = Some v
+        /\ valid_val v t.
+
+  Definition compat_menv (me: menv) (env: Clight.env) (m: Memory.Mem.mem):  Prop :=
+    forall x t v,
+      mfind_mem x me = Some v ->
+      exists co loc' loc ofs delta,
+        Ctypes.field_offset (Clight.genv_cenv tge) x (Ctypes.co_members co) = Errors.OK delta
+        /\ Memory.Mem.load (chunk_of_typ t) m loc (Int.unsigned (Int.add ofs (Int.repr delta))) = Some v
+        /\ valid_val v t
+        /\ Maps.PTree.get main_node (Clight.genv_cenv tge) = Some co 
+        /\ Maps.PTree.get self_id env = Some (loc', pointer_of_node main_node)
+        /\ Memory.Mem.load (chunk_of_typ (pointer_of_node main_node)) m loc' 0 = Some (Values.Vptr loc ofs)
+        /\ Ctypes.access_mode (pointer_of_node main_node) = Ctypes.By_value (chunk_of_typ (pointer_of_node main_node)).
+  
+  Hint Constructors Clight.eval_lvalue Clight.eval_expr well_typed.
+
+  Lemma expr_eval':
+    forall me ve exp v e le m,
+      compat_venv ve e m ->
+      compat_menv me e m ->
+      exp_eval me ve exp v ->
+      Clight.eval_expr tge e le m (translate_exp main_node exp) v.
+  Proof.
+    intros me ve exp;
+    induction exp as [x ty|x ty|c ty];
+    intros ** Hvenv Hmenv Heval;
+    inversion_clear Heval as [? ? ? Hmto|? ? ? Hmem|];
+    subst; simpl.
+    - destruct (Hvenv _ ty _ Hmto) as [loc [? [? [? []]]]].
+      apply Clight.eval_Elvalue with (loc:=loc) (ofs:=Int.zero); auto.
+      eapply Clight.deref_loc_value; eauto.
+    - destruct (Hmenv _ ty _ Hmem)
+        as [co [loc' [loc [ofs [delta [? [? [[] [? [? [? []]]]]]]]]]]].  
+      apply Clight.eval_Elvalue
+      with (loc:=loc) (ofs:=Int.add ofs (Int.repr delta)).
+      + apply Clight.eval_Efield_struct
+        with (id:=main_node) (co:=co) (att:=Ctypes.noattr); auto.
+        apply Clight.eval_Elvalue with (loc:=loc) (ofs:=ofs). 
+        * apply Clight.eval_Ederef. 
+          apply Clight.eval_Elvalue with (loc:=loc') (ofs:=Int.zero); eauto.
+          apply Clight.deref_loc_value with (chunk:=AST.Mint32); eauto.
+        * now apply Clight.deref_loc_copy.
+      + eapply Clight.deref_loc_value; eauto. 
+    - destruct c; constructor.
   Qed.
-              
-  Theorem simu:
+
+  Definition compat_vars (env: Clight.env): Prop :=
+    forall x t,
+      In (x, t) prog.(p_vars) ->
+      exists loc,
+        Maps.PTree.get x env = Some (loc, t).
+
+  Definition compat_fields (env: Clight.env) (m: Memory.Mem.mem): Prop :=
+    forall x t,
+      wt_state_pred (x, t) prog ->
+      exists co loc' loc ofs delta,
+        Ctypes.field_offset (Clight.genv_cenv tge) x (Ctypes.co_members co) = Errors.OK delta
+        /\ Maps.PTree.get main_node (Clight.genv_cenv tge) = Some co
+        /\ Maps.PTree.get self_id env = Some (loc', pointer_of_node main_node)
+        /\ Memory.Mem.load (chunk_of_typ (pointer_of_node main_node)) m loc' 0 = Some (Values.Vptr loc ofs).
+
+  Inductive match_states': state -> Clight.state -> Prop :=
+    state_intro': forall me ve s k e le m,
+      compat_venv ve e m ->
+      compat_menv me e m ->
+      compat_vars e ->
+      compat_fields e m ->
+      well_typed s ->
+      match_states'
+        (me, ve, s)
+        (Clight.State main_fun (translate_stmt main_node s) k e le m).
+
+   Lemma compat_venv_pres:
+    forall ve me e m x v t loc,
+      compat_venv ve e m ->
+      compat_menv me e m ->
+      compat_fields e m ->
+      Maps.PTree.get x e = Some (loc, t) ->
+      exists m',
+        Memory.Mem.store (chunk_of_typ t) m loc 0 v = Some m' 
+        /\ valid_val v t
+        /\ compat_venv (PM.add x v ve) e m'
+        /\ compat_menv me e m'
+        /\ compat_fields e m'.
+  Proof.
+    intros ** Hvenv Hmenv Hfields Hget.
+    assert (Memory.Mem.valid_access m (chunk_of_typ t) loc 0 Memtype.Writable) as H. admit.
+    destruct (Memory.Mem.valid_access_store m (chunk_of_typ t) loc 0 v H) as [m'].
+    exists m'. repeat split; auto.
+  Admitted.
+
+  Lemma compat_menv_pres:
+    forall ve me e m x v t loc ofs delta,
+      compat_venv ve e m ->
+      compat_menv me e m ->
+      compat_fields e m ->
+      (* Maps.PTree.get x e = Some (loc, t) -> *)
+      exists m',
+        Memory.Mem.store (chunk_of_typ t) m loc (Int.unsigned (Int.add ofs (Int.repr delta))) v = Some m'
+        /\ valid_val v t
+        /\ compat_venv ve e m'
+        /\ compat_menv (madd_mem x v me) e m'
+        /\ compat_fields e m'.
+  Proof.
+    admit.
+  Qed.
+
+  (*Theorem simu:
     forall S1 S2,
       stmt_eval prog S1 S2 ->
       forall S1',
@@ -559,22 +685,22 @@ Section PRESERVATION.
             /\ match_states S2 S2'.
   Proof.
     induction 1 as [? ? ? ? ? ? ? Heval Hve(* |? ? ? ? ? ? ? Heval Hmem *)];
-    inversion_clear 1 as [? ? ? ? env ? ? Hvars Hwt Hwa]; simpl.
-    - assert (m': Memory.Mem.mem). admit. (* memory state after statement step *)
-      exists (Clight.State main_fun Clight.Sskip k env lenv m'); exists Events.E0; split.
+    inversion_clear 1 as [? ? ? ? env ? ? Hvars Hwt Hwa Hwe Hmem]; simpl.
+    - exists (Clight.State main_fun Clight.Sskip k env lenv (compat_mem me ve')); exists Events.E0; split.
       + apply Smallstep.plus_one.
         unfold Clight.step1.
-        assert (Ctypes.access_mode (typeof e) = Ctypes.By_value (AST.chunk_of_type (Ctypes.typ_of_type (typeof e)))). admit.
-        assert (v <> Values.Vundef) as V. admit.
-        inv Hwt.
-        inv Hwa.
+        inversion_clear Hwe as [? ? ? ? Hwe'|].
+        inversion_clear Hwe' as [? ? ? v' Haccess Hv Ht Hload Heval'].
+        pose proof exp_eval_det as Hdet; generalize (Hdet _ _ _ _ _ Heval' Heval).
+        intro; subst.
+        inversion_clear Hwt as [? ? Hwt'|].
+        inversion_clear Hwa as [? ? ? ? loc Hwa' Hget|].
         apply Clight.step_assign with (loc:=loc) (ofs:=Int.zero) (v2:=v) (v:=v); auto.
-        * eapply expr_eval; eauto. admit. (*  *)
+        * eapply expr_eval; eauto. 
         * rewrite type_pres; simpl.
           eapply sem_cast_same; eauto.
-          eapply type_of_val; eauto. (* seems pretty wrong... *)
         * eapply Clight.assign_loc_value; eauto. 
-          simpl. admit.         (* STORE *)
+          inversion_clear Hwa'; simpl; auto.
       + now constructor.
     (* - assert (m': Memory.Mem.mem). admit. (* memory state after statement step *) *)
     (*   assert (loc: Values.block). admit. *)
@@ -608,4 +734,51 @@ Section PRESERVATION.
     (*     * eapply Clight.assign_loc_value; eauto.  *)
     (*       simpl. admit.         (* STORE *) *)
     (*   + now constructor. *)
+  Qed.*)
+
+  Theorem simu':
+    forall S1 S2,
+      stmt_eval prog S1 S2 ->
+      forall S1',
+        match_states' S1 S1' ->
+        exists S2' t,
+            Smallstep.plus Clight.step1 tge S1' t S2'
+            /\ match_states' S2 S2'.
+  Proof.
+    induction 1;
+    inversion_clear 1 as [? ? ? ? ? ? ? Hvenv Hmenv Hvars Hfields Hwt]; 
+    inversion_clear Hwt as [? ? Hin|? ? Hpred|];
+    subst; simpl.
+
+    (* Assign x e : "x = e" *)
+    - destruct (Hvars _ _ Hin) as [loc Hget].
+      destruct (compat_venv_pres _ _ _ _ x v (typeof e) loc Hvenv Hmenv Hfields Hget)
+        as [m' [? [[? []] [? []]]]];
+      exists (Clight.State main_fun Clight.Sskip k e0 le m'); exists Events.E0; split.
+      + apply Smallstep.plus_one, Clight.step_assign
+        with (loc:=loc) (ofs:=Int.zero) (v2:=v) (v:=v); auto.
+        * eapply expr_eval'; eauto. 
+        * rewrite type_pres; eapply sem_cast_same; eauto. 
+        * eapply Clight.assign_loc_value; eauto. 
+      + constructor; auto. 
+
+    (* AssignSt x e : "self->x = e"*)
+    - destruct (Hfields _ _ Hpred) as [co [loc' [loc [ofs [delta [? [? []]]]]]]];
+      destruct (compat_menv_pres _ _ _ _ x v (typeof e) loc ofs delta Hvenv Hmenv Hfields)
+        as [m' [? [[? []] [? []]]]].
+      exists (Clight.State main_fun Clight.Sskip k e0 le m'); exists Events.E0; split.
+      + apply Smallstep.plus_one, Clight.step_assign
+        with (loc:=loc) (ofs:=Int.add ofs (Int.repr delta)) (v2:=v) (v:=v).
+        *{ apply Clight.eval_Efield_struct
+           with (id:=main_node) (co:=co) (att:=Ctypes.noattr); auto.
+           apply Clight.eval_Elvalue with (loc:=loc) (ofs:=ofs). 
+           - apply Clight.eval_Ederef. 
+             apply Clight.eval_Elvalue with (loc:=loc') (ofs:=Int.zero); eauto.
+             apply Clight.deref_loc_value with (chunk:=AST.Mint32); eauto.
+           - now apply Clight.deref_loc_copy.
+         }
+        * eapply expr_eval'; eauto. 
+        * rewrite type_pres; eapply sem_cast_same; eauto. 
+        * eapply Clight.assign_loc_value; eauto.
+      + constructor; auto. 
   Qed.
